# baseURI: https://w3id.org/isample/1.0/esmaterialsample/essampletype
# imports: http://www.w3.org/2004/02/skos/core
# imports: https://w3id.org/isample/vocabulary/specimentype/1.0/specimentypevocabulary

@prefix dcterm: <http://purl.org/dc/terms/> .
@prefix esmat: <https://w3id.org/isample/1.0/esmaterialsample/> .
@prefix owl: <http://www.w3.org/2002/07/owl#> .
@prefix rdf: <http://www.w3.org/1999/02/22-rdf-syntax-ns#> .
@prefix rdfs: <http://www.w3.org/2000/01/rdf-schema#> .
@prefix schema: <https://schema.org/> .
@prefix sdev: <http://vocab.nerc.ac.uk/collection/L05/current/> .
@prefix sdo: <http://schema.org/> .
@prefix skos: <http://www.w3.org/2004/02/skos/core#> .
@prefix spec: <https://w3id.org/isample/vocabulary/specimentype/1.0/> .
@prefix xsd: <http://www.w3.org/2001/XMLSchema#> .

<AWDID:2004562>
  rdf:type schema:Grant ;
  schema:funder <https://ror.org/04nh1dc89> ;
  schema:name "Collaborative Research: Frameworks: Internet of Samples: Toward an Interdisciplinary Cyberinfrastructure for Material Samples" ;
  schema:url "https://nsf.gov/awardsearch/showAward?AWD_ID=2004562" ;
.
<http://www.w3.org/2004/02/skos/core>
  rdf:type owl:Ontology ;
  dcterm:contributor "Dave Beckett" ;
  dcterm:contributor "Nikki Rogers" ;
  dcterm:contributor "Participants in W3C's Semantic Web Deployment Working Group." ;
  dcterm:creator "Alistair Miles" ;
  dcterm:creator "Sean Bechhofer" ;
  dcterm:description "An RDF vocabulary for describing the basic structure and content of concept schemes such as thesauri, classification schemes, subject heading lists, taxonomies, 'folksonomies', other types of controlled vocabulary, and also concept schemes embedded in glossaries and terminologies."@en ;
  dcterm:title "SKOS Vocabulary"@en ;
  rdfs:label "SKOS Core RDF vocabulary" ;
  rdfs:seeAlso <http://www.w3.org/TR/skos-reference/> ;
  owl:versionInfo "Modified by TopQuadrant to assert three rdfs:subClassOf owl:Thing triples." ;
.
skos:Collection
  rdf:type owl:Class ;
  rdfs:isDefinedBy <http://www.w3.org/2004/02/skos/core> ;
  rdfs:label "Collection"@en ;
  rdfs:subClassOf owl:Thing ;
  owl:disjointWith skos:Concept ;
  owl:disjointWith skos:ConceptScheme ;
  skos:definition "A meaningful collection of concepts."@en ;
  skos:scopeNote "Labelled collections can be used where you would like a set of concepts to be displayed under a 'node label' in the hierarchy."@en ;
.
skos:Concept
  rdf:type owl:Class ;
  rdfs:isDefinedBy <http://www.w3.org/2004/02/skos/core> ;
  rdfs:label "Concept"@en ;
  rdfs:subClassOf owl:Thing ;
  skos:definition "An idea or notion; a unit of thought."@en ;
.
skos:ConceptScheme
  rdf:type owl:Class ;
  rdfs:isDefinedBy <http://www.w3.org/2004/02/skos/core> ;
  rdfs:label "Concept Scheme"@en ;
  rdfs:subClassOf owl:Thing ;
  owl:disjointWith skos:Concept ;
  skos:definition "A set of concepts, optionally including statements about semantic relationships between those concepts."@en ;
  skos:example "Thesauri, classification schemes, subject heading lists, taxonomies, 'folksonomies', and other types of controlled vocabulary are all examples of concept schemes. Concept schemes are also embedded in glossaries and terminologies."@en ;
  skos:scopeNote "A concept scheme may be defined to include concepts from different sources."@en ;
.
skos:OrderedCollection
  rdf:type owl:Class ;
  rdfs:isDefinedBy <http://www.w3.org/2004/02/skos/core> ;
  rdfs:label "Ordered Collection"@en ;
  rdfs:subClassOf skos:Collection ;
  skos:definition "An ordered collection of concepts, where both the grouping and the ordering are meaningful."@en ;
  skos:scopeNote "Ordered collections can be used where you would like a set of concepts to be displayed in a specific order, and optionally under a 'node label'."@en ;
.
skos:altLabel
  rdf:type rdf:Property ;
  rdf:type owl:AnnotationProperty ;
  rdfs:comment "The range of skos:altLabel is the class of RDF plain literals."@en ;
  rdfs:comment "skos:prefLabel, skos:altLabel and skos:hiddenLabel are pairwise disjoint properties."@en ;
  rdfs:isDefinedBy <http://www.w3.org/2004/02/skos/core> ;
  rdfs:label "alternative label"@en ;
  rdfs:subPropertyOf rdfs:label ;
  skos:definition "An alternative lexical label for a resource."@en ;
  skos:example "Acronyms, abbreviations, spelling variants, and irregular plural/singular forms may be included among the alternative labels for a concept. Mis-spelled terms are normally included as hidden labels (see skos:hiddenLabel)."@en ;
.
skos:broadMatch
  rdf:type rdf:Property ;
  rdf:type owl:ObjectProperty ;
  rdfs:isDefinedBy <http://www.w3.org/2004/02/skos/core> ;
  rdfs:label "has broader match"@en ;
  rdfs:subPropertyOf skos:broader ;
  rdfs:subPropertyOf skos:mappingRelation ;
  owl:inverseOf skos:narrowMatch ;
  skos:definition "skos:broadMatch is used to state a hierarchical mapping link between two conceptual resources in different concept schemes."@en ;
.
skos:broader
  rdf:type rdf:Property ;
  rdf:type owl:ObjectProperty ;
  rdfs:comment "Broader concepts are typically rendered as parents in a concept hierarchy (tree)."@en ;
  rdfs:isDefinedBy <http://www.w3.org/2004/02/skos/core> ;
  rdfs:label "has broader"@en ;
  rdfs:subPropertyOf skos:broaderTransitive ;
  owl:inverseOf skos:narrower ;
  skos:definition "Relates a concept to a concept that is more general in meaning."@en ;
  skos:scopeNote "By convention, skos:broader is only used to assert an immediate (i.e. direct) hierarchical link between two conceptual resources."@en ;
.
skos:broaderTransitive
  rdf:type rdf:Property ;
  rdf:type owl:ObjectProperty ;
  rdf:type owl:TransitiveProperty ;
  rdfs:isDefinedBy <http://www.w3.org/2004/02/skos/core> ;
  rdfs:label "has broader transitive"@en ;
  rdfs:subPropertyOf skos:semanticRelation ;
  owl:inverseOf skos:narrowerTransitive ;
  skos:definition "skos:broaderTransitive is a transitive superproperty of skos:broader." ;
  skos:scopeNote "By convention, skos:broaderTransitive is not used to make assertions. Rather, the properties can be used to draw inferences about the transitive closure of the hierarchical relation, which is useful e.g. when implementing a simple query expansion algorithm in a search application."@en ;
.
skos:changeNote
  rdf:type rdf:Property ;
  rdf:type owl:AnnotationProperty ;
  rdfs:isDefinedBy <http://www.w3.org/2004/02/skos/core> ;
  rdfs:label "change note"@en ;
  rdfs:subPropertyOf skos:note ;
  skos:definition "A note about a modification to a concept."@en ;
.
skos:closeMatch
  rdf:type rdf:Property ;
  rdf:type owl:ObjectProperty ;
  rdf:type owl:SymmetricProperty ;
  rdfs:isDefinedBy <http://www.w3.org/2004/02/skos/core> ;
  rdfs:label "has close match"@en ;
  rdfs:subPropertyOf skos:mappingRelation ;
  skos:definition "skos:closeMatch is used to link two concepts that are sufficiently similar that they can be used interchangeably in some information retrieval applications. In order to avoid the possibility of \"compound errors\" when combining mappings across more than two concept schemes, skos:closeMatch is not declared to be a transitive property."@en ;
.
skos:definition
  rdf:type rdf:Property ;
  rdf:type owl:AnnotationProperty ;
  rdfs:isDefinedBy <http://www.w3.org/2004/02/skos/core> ;
  rdfs:label "definition"@en ;
  rdfs:subPropertyOf skos:note ;
  skos:definition "A statement or formal explanation of the meaning of a concept."@en ;
.
skos:editorialNote
  rdf:type rdf:Property ;
  rdf:type owl:AnnotationProperty ;
  rdfs:isDefinedBy <http://www.w3.org/2004/02/skos/core> ;
  rdfs:label "editorial note"@en ;
  rdfs:subPropertyOf skos:note ;
  skos:definition "A note for an editor, translator or maintainer of the vocabulary."@en ;
.
skos:exactMatch
  rdf:type rdf:Property ;
  rdf:type owl:ObjectProperty ;
  rdf:type owl:SymmetricProperty ;
  rdf:type owl:TransitiveProperty ;
  rdfs:comment "skos:exactMatch is disjoint with each of the properties skos:broadMatch and skos:relatedMatch."@en ;
  rdfs:isDefinedBy <http://www.w3.org/2004/02/skos/core> ;
  rdfs:label "has exact match"@en ;
  rdfs:subPropertyOf skos:closeMatch ;
  skos:definition "skos:exactMatch is used to link two concepts, indicating a high degree of confidence that the concepts can be used interchangeably across a wide range of information retrieval applications. skos:exactMatch is a transitive property, and is a sub-property of skos:closeMatch."@en ;
.
skos:example
  rdf:type rdf:Property ;
  rdf:type owl:AnnotationProperty ;
  rdfs:isDefinedBy <http://www.w3.org/2004/02/skos/core> ;
  rdfs:label "example"@en ;
  rdfs:subPropertyOf skos:note ;
  skos:definition "An example of the use of a concept."@en ;
.
skos:hasTopConcept
  rdf:type rdf:Property ;
  rdf:type owl:ObjectProperty ;
  rdfs:domain skos:ConceptScheme ;
  rdfs:isDefinedBy <http://www.w3.org/2004/02/skos/core> ;
  rdfs:label "has top concept"@en ;
  rdfs:range skos:Concept ;
  owl:inverseOf skos:topConceptOf ;
  skos:definition "Relates, by convention, a concept scheme to a concept which is topmost in the broader/narrower concept hierarchies for that scheme, providing an entry point to these hierarchies."@en ;
.
skos:hiddenLabel
  rdf:type rdf:Property ;
  rdf:type owl:AnnotationProperty ;
  rdfs:comment "The range of skos:hiddenLabel is the class of RDF plain literals."@en ;
  rdfs:comment "skos:prefLabel, skos:altLabel and skos:hiddenLabel are pairwise disjoint properties."@en ;
  rdfs:isDefinedBy <http://www.w3.org/2004/02/skos/core> ;
  rdfs:label "hidden label"@en ;
  rdfs:subPropertyOf rdfs:label ;
  skos:definition "A lexical label for a resource that should be hidden when generating visual displays of the resource, but should still be accessible to free text search operations."@en ;
.
skos:historyNote
  rdf:type rdf:Property ;
  rdf:type owl:AnnotationProperty ;
  rdfs:isDefinedBy <http://www.w3.org/2004/02/skos/core> ;
  rdfs:label "history note"@en ;
  rdfs:subPropertyOf skos:note ;
  skos:definition "A note about the past state/use/meaning of a concept."@en ;
.
skos:inScheme
  rdf:type rdf:Property ;
  rdf:type owl:ObjectProperty ;
  rdfs:isDefinedBy <http://www.w3.org/2004/02/skos/core> ;
  rdfs:label "is in scheme"@en ;
  rdfs:range skos:ConceptScheme ;
  rdfs:subPropertyOf skos:member ;
  skos:definition "Relates a resource (for example a concept) to a concept scheme in which it is included."@en ;
  skos:scopeNote "A concept may be a member of more than one concept scheme."@en ;
.
skos:mappingRelation
  rdf:type rdf:Property ;
  rdf:type owl:ObjectProperty ;
  rdfs:comment "These concept mapping relations mirror semantic relations, and the data model defined below is similar (with the exception of skos:exactMatch) to the data model defined for semantic relations. A distinct vocabulary is provided for concept mapping relations, to provide a convenient way to differentiate links within a concept scheme from links between concept schemes. However, this pattern of usage is not a formal requirement of the SKOS data model, and relies on informal definitions of best practice."@en ;
  rdfs:isDefinedBy <http://www.w3.org/2004/02/skos/core> ;
  rdfs:label "is in mapping relation with"@en ;
  rdfs:subPropertyOf skos:semanticRelation ;
  skos:definition "Relates two concepts coming, by convention, from different schemes, and that have comparable meanings"@en ;
.
skos:member
  rdf:type rdf:Property ;
  rdf:type owl:ObjectProperty ;
  rdfs:domain skos:Collection ;
  rdfs:isDefinedBy <http://www.w3.org/2004/02/skos/core> ;
  rdfs:label "has member"@en ;
  rdfs:range [
      rdf:type owl:Class ;
      owl:unionOf (
          skos:Concept
          skos:Collection
        ) ;
    ] ;
  skos:definition "Relates a collection to one of its members."@en ;
.
skos:memberList
  rdf:type rdf:Property ;
  rdf:type owl:FunctionalProperty ;
  rdf:type owl:ObjectProperty ;
  rdfs:comment """For any resource, every item in the list given as the value of the
      skos:memberList property is also a value of the skos:member property."""@en ;
  rdfs:domain skos:OrderedCollection ;
  rdfs:isDefinedBy <http://www.w3.org/2004/02/skos/core> ;
  rdfs:label "has member list"@en ;
  rdfs:range rdf:List ;
  skos:definition "Relates an ordered collection to the RDF list containing its members."@en ;
.
skos:narrowMatch
  rdf:type rdf:Property ;
  rdf:type owl:ObjectProperty ;
  rdfs:isDefinedBy <http://www.w3.org/2004/02/skos/core> ;
  rdfs:label "has narrower match"@en ;
  rdfs:subPropertyOf skos:mappingRelation ;
  rdfs:subPropertyOf skos:narrower ;
  owl:inverseOf skos:broadMatch ;
  skos:definition "skos:narrowMatch is used to state a hierarchical mapping link between two conceptual resources in different concept schemes."@en ;
.
skos:narrower
  rdf:type rdf:Property ;
  rdf:type owl:ObjectProperty ;
  rdfs:comment "Narrower concepts are typically rendered as children in a concept hierarchy (tree)."@en ;
  rdfs:isDefinedBy <http://www.w3.org/2004/02/skos/core> ;
  rdfs:label "has narrower"@en ;
  rdfs:subPropertyOf skos:narrowerTransitive ;
  owl:inverseOf skos:broader ;
  skos:definition "Relates a concept to a concept that is more specific in meaning."@en ;
  skos:scopeNote "By convention, skos:broader is only used to assert an immediate (i.e. direct) hierarchical link between two conceptual resources."@en ;
.
skos:narrowerTransitive
  rdf:type rdf:Property ;
  rdf:type owl:ObjectProperty ;
  rdf:type owl:TransitiveProperty ;
  rdfs:isDefinedBy <http://www.w3.org/2004/02/skos/core> ;
  rdfs:label "has narrower transitive"@en ;
  rdfs:subPropertyOf skos:semanticRelation ;
  owl:inverseOf skos:broaderTransitive ;
  skos:definition "skos:narrowerTransitive is a transitive superproperty of skos:narrower." ;
  skos:scopeNote "By convention, skos:narrowerTransitive is not used to make assertions. Rather, the properties can be used to draw inferences about the transitive closure of the hierarchical relation, which is useful e.g. when implementing a simple query expansion algorithm in a search application."@en ;
.
skos:notation
  rdf:type rdf:Property ;
  rdf:type owl:DatatypeProperty ;
  rdfs:isDefinedBy <http://www.w3.org/2004/02/skos/core> ;
  rdfs:label "notation"@en ;
  skos:definition "A notation, also known as classification code, is a string of characters such as \"T58.5\" or \"303.4833\" used to uniquely identify a concept within the scope of a given concept scheme."@en ;
  skos:scopeNote "By convention, skos:notation is used with a typed literal in the object position of the triple."@en ;
.
skos:note
  rdf:type rdf:Property ;
  rdf:type owl:AnnotationProperty ;
  rdfs:isDefinedBy <http://www.w3.org/2004/02/skos/core> ;
  rdfs:label "note"@en ;
  rdfs:subPropertyOf rdfs:seeAlso ;
  skos:definition "A general note, for any purpose."@en ;
  skos:scopeNote "This property may be used directly, or as a super-property for more specific note types."@en ;
.
skos:prefLabel
  rdf:type rdf:Property ;
  rdf:type owl:AnnotationProperty ;
  rdfs:comment "A resource has no more than one value of skos:prefLabel per language tag."@en ;
  rdfs:comment "The range of skos:prefLabel is the class of RDF plain literals."@en ;
  rdfs:comment """skos:prefLabel, skos:altLabel and skos:hiddenLabel are pairwise
      disjoint properties."""@en ;
  rdfs:isDefinedBy <http://www.w3.org/2004/02/skos/core> ;
  rdfs:label "preferred label"@en ;
  rdfs:subPropertyOf rdfs:label ;
  skos:definition "The preferred lexical label for a resource, in a given language."@en ;
.
skos:related
  rdf:type rdf:Property ;
  rdf:type owl:ObjectProperty ;
  rdf:type owl:SymmetricProperty ;
  rdfs:comment "skos:related is disjoint with skos:broaderTransitive"@en ;
  rdfs:isDefinedBy <http://www.w3.org/2004/02/skos/core> ;
  rdfs:label "has related"@en ;
  rdfs:subPropertyOf skos:semanticRelation ;
  skos:definition "Relates a concept to a concept with which there is an associative semantic relationship."@en ;
.
skos:relatedMatch
  rdf:type rdf:Property ;
  rdf:type owl:ObjectProperty ;
  rdf:type owl:SymmetricProperty ;
  rdfs:isDefinedBy <http://www.w3.org/2004/02/skos/core> ;
  rdfs:label "has related match"@en ;
  rdfs:subPropertyOf skos:mappingRelation ;
  rdfs:subPropertyOf skos:related ;
  skos:definition "skos:relatedMatch is used to state an associative mapping link between two conceptual resources in different concept schemes."@en ;
.
skos:scopeNote
  rdf:type rdf:Property ;
  rdf:type owl:AnnotationProperty ;
  rdfs:isDefinedBy <http://www.w3.org/2004/02/skos/core> ;
  rdfs:label "scope note"@en ;
  rdfs:subPropertyOf skos:note ;
  skos:definition "A note that helps to clarify the meaning and/or the use of a concept."@en ;
.
skos:semanticRelation
  rdf:type rdf:Property ;
  rdf:type owl:ObjectProperty ;
  rdfs:domain skos:Concept ;
  rdfs:isDefinedBy <http://www.w3.org/2004/02/skos/core> ;
  rdfs:label "is in semantic relation with"@en ;
  rdfs:range skos:Concept ;
  skos:definition "Links a concept to a concept related by meaning."@en ;
  skos:scopeNote "This property should not be used directly, but as a super-property for all properties denoting a relationship of meaning between concepts."@en ;
.
skos:topConceptOf
  rdf:type rdf:Property ;
  rdf:type owl:ObjectProperty ;
  rdfs:domain skos:Concept ;
  rdfs:isDefinedBy <http://www.w3.org/2004/02/skos/core> ;
  rdfs:label "is top concept in scheme"@en ;
  rdfs:range skos:ConceptScheme ;
  rdfs:subPropertyOf skos:inScheme ;
  owl:inverseOf skos:hasTopConcept ;
  skos:definition "Relates a concept to the concept scheme that it is a top level concept of."@en ;
.
esmat:boxedcore
  rdf:type skos:Concept ;
  dcterm:source "this vocabulary" ;
  rdfs:isDefinedBy esmat:essampletype ;
  rdfs:label "Boxed core"@en ;
  skos:broader spec:genericaggregation ;
  skos:definition "A collection of core peices that are stored in an individual box. Typically the box will contain core peices from the same core."@en ;
  skos:inScheme esmat:essampletype ;
  skos:prefLabel "Boxed core"@en ;
.
esmat:cellculture
  rdf:type skos:Concept ;
  dcterm:source "https://en.wikipedia.org/wiki/Cell_culture" ;
  rdfs:isDefinedBy esmat:essampletype ;
  rdfs:label "Cell culture"@en ;
  skos:broader spec:analyticalpreparation ;
  skos:broader spec:bundlebiomeaggregation ;
  skos:definition "a collection of cells are grown under controlled conditions, generally outside of their natural environment"@en ;
  skos:inScheme esmat:essampletype ;
  skos:prefLabel "Cell culture"@en ;
.
esmat:chipchannelsample
  rdf:type skos:Concept ;
  dcterm:source "http://earthsci.org/mineral/rockmin/sampling/sampling.html#Rock%20Sampling" ;
  rdfs:isDefinedBy esmat:essampletype ;
  rdfs:label "Chip Channel Sample"@en ;
  skos:broader esmat:compositesample ;
  skos:definition "small chips of rock collected over a specified interval, with the objective to obtain a representative sample for that interval. Most of the time chip channel samples are collected in succession along a sample line which is laid out in advance using a tape.  The freshest material possible is sampled, preferably chipping directly from bedrock. Sample intervals are set at a specified width, usually ranging from 30cm to 7m. Due to the method of sampling, chip channel samples tend to be rather large (up to 20 pounds for a five foot interval)"@en ;
  skos:inScheme esmat:essampletype ;
  skos:prefLabel "Chip Channel Sample"@en ;
.
esmat:compositesample
  rdf:type skos:Concept ;
  dcterm:source "this vocabulary" ;
  rdfs:label "Composite sample"@en ;  rdfs:isDefinedBy esmat:essampletype ;
  skos:broader spec:genericaggregation ;
  skos:definition "a sample composed of multiple peices, representative of some material, or representative of some site. The peices do not all originate from the same object."@en ;
  skos:prefLabel "Composite sample"@en ;  skos:inScheme esmat:essampletype ;
.
esmat:core
  rdf:type skos:Concept ;
  dcterm:source "this vocabulary" ;
  rdfs:isDefinedBy esmat:essampletype ;
  rdfs:label "Core"@en ;
  skos:broader spec:solidmaterialspecimen ;
  skos:definition "Cylinder of rock or sediment extracted from within the earth, and representing the entire sample extracted during a single borehole drilling event.  Typically using some rotary drilling technology. In many cases the core is extracted in segments that are 'core sections'. A core from a single borehole is rarely a continous unbroken object; commonly parts of the core will break up during drilling or extraction, leaving gaps or sections that are granular material. Cores are normally composed of consolidated ('solid') material, but in some cases loosely consolidated material might be recovered, and considered sediment or tephra. To be called 'core' the material must be sufficiently consolidated to maintain a cylindrical shape. A core hasPart (hasChild) 'Core section'"@en ;
  skos:inScheme esmat:essampletype ;
  skos:prefLabel "Core"@en ;
.
esmat:corecatcher
  rdf:type skos:Concept ;
  dcterm:source "https://www.geosamples.org/vocabularies/sample-type-object" ;
  rdfs:isDefinedBy esmat:essampletype ;
  rdfs:label "Core Catcher"@en ;
  skos:broader spec:genericaggregation ;
  skos:definition "material recovered from the core catcher of a sedimentary core and which is treated as a separate section from the core. The core catcher is a device at the bottom of the core barrel that prevents the core from sliding out while the barrel is retrieved from the hole. (http://publications.iodp.org/proceedings/323/102/102_.htm)"@en ;
  skos:inScheme esmat:essampletype ;
  skos:prefLabel "Core Catcher"@en ;
.
esmat:corehalfround
  rdf:type skos:Concept ;
  dcterm:source "https://www.geosamples.org/vocabularies/sample-type-object" ;
  rdfs:isDefinedBy esmat:essampletype ;
  rdfs:label "Core half round"@en ;
  skos:broader spec:solidmaterialspecimen ;
  skos:definition "Half-cylindrical peice of consolidated material produced by along-axis split of a core whole round along a selected diameter .    Has childOf relation to core section or core, core section, or Core peice from which is was split"@en ;
  skos:inScheme esmat:essampletype ;
  skos:prefLabel "Core half round"@en ;
.
esmat:corepeice
  rdf:type skos:Concept ;
  dcterm:source "https://www.geosamples.org/vocabularies/sample-type-object" ;
  rdfs:isDefinedBy esmat:essampletype ;
  rdfs:label "Core peice"@en ;
  skos:broader spec:solidmaterialspecimen ;
  skos:definition "A cylindrical peice of consolidated earth material extracted as a single solid object between breaks in recovery of core from a borehole. has parent core section"@en ;
  skos:inScheme esmat:essampletype ;
  skos:prefLabel "Core peice"@en ;
.
esmat:corequarterround
  rdf:type skos:Concept ;
  dcterm:source "https://www.geosamples.org/vocabularies/sample-type-object" ;
  rdfs:isDefinedBy esmat:essampletype ;
  rdfs:label "Core quarter round"@en ;
  skos:broader spec:solidmaterialspecimen ;
  skos:definition "a partial cylindrical peice of consolidated material created by along-axis split of a core half round. Has Parent core half round"@en ;
  skos:inScheme esmat:essampletype ;
  skos:prefLabel "Core quarter round"@en ;
.
esmat:coresection
  rdf:type skos:Concept ;
  dcterm:source "https://www.geosamples.org/vocabularies" ;
  rdfs:isDefinedBy esmat:essampletype ;
  rdfs:label "Core section"@en ;
  skos:broader spec:solidmaterialspecimen ;
  skos:definition "Segment of a core representing some interval along the well bore. Child of Core"@en ;
  skos:inScheme esmat:essampletype ;
  skos:prefLabel "Core section"@en ;
.
esmat:coresubpeice
  rdf:type skos:Concept ;
  dcterm:source "https://www.geosamples.org/vocabularies" ;
  rdfs:isDefinedBy esmat:essampletype ;
  rdfs:label "Core subpeice"@en ;
  skos:broader spec:solidmaterialspecimen ;
  skos:definition "A peice of consolidated material broken from a core peice. has Parent core peice or core section"@en ;
  skos:inScheme esmat:essampletype ;
  skos:prefLabel "Core subpeice"@en ;
.
esmat:cuttings
  rdf:type skos:Concept ;
  dcterm:source "http://vocabulary.odm2.org/specimentype/cuttings/" ;
  rdfs:isDefinedBy esmat:essampletype ;
  rdfs:label "Cuttings"@en ;
  skos:broader spec:genericaggregation ;
  skos:definition "unconsolidated Earth material produced by the grinding action of a drill bit during drilling of a borehole."@en ;
  skos:inScheme esmat:essampletype ;
  skos:prefLabel "Cuttings"@en ;
.
esmat:directfluidsample
  rdf:type skos:Concept ;
  dcterm:source "this vocabulary" ;
  rdfs:label "Direct fluid sample"@en ;
  skos:broader spec:fluidincontainer ;  rdfs:isDefinedBy esmat:essampletype ;
  skos:definition "a fluid collected from the sampled feature (e.g. water body, hydrothermal vent, atmosphere...) with no processing. (e.g. filtration, addition of preservatives)."@en ;
  skos:prefLabel "Direct fluid sample"@en ;  skos:inScheme esmat:essampletype ;
.
esmat:dissolvedchemicalfraction
  rdf:type skos:Concept ;
  dcterm:source "" ;
  rdfs:isDefinedBy esmat:essampletype ;
  rdfs:label "Dissolved chemical fraction"@en ;
  skos:broader spec:analyticalpreparation ;
  skos:broader spec:fluidincontainer ;
  skos:definition "A fluid concentrating some constituent of interest from a parent sample. The dissolved constituent is actually the sample material of interest."@en ;
  skos:inScheme esmat:essampletype ;
  skos:prefLabel "Dissolved chemical fraction"@en ;
.
esmat:dredge
  rdf:type skos:Concept ;
  dcterm:source "https://www.geosamples.org/vocabularies/sample-type-object" ;
  rdfs:isDefinedBy esmat:essampletype ;
  rdfs:label "Dredge"@en ;
  skos:broader spec:genericaggregation ;
  skos:definition "an aggregation of material sampled by dragging a collection bucket (dredge) across the bottom of a water body"@en ;
  skos:inScheme esmat:essampletype ;
  skos:prefLabel "Dredge"@en ;
.
esmat:dustwipe
  rdf:type skos:Concept ;
  dcterm:source "https://www.cdc.gov/nceh/lead/docs/publications/Environmental_Sampling.pdf, dust wipe sampling" ;
  rdfs:isDefinedBy esmat:essampletype ;
  rdfs:label "Dust wipe"@en ;
  skos:broader spec:othersolidobject ;
  skos:definition "a pre-weighed and packaged paper towel (wipe) used to wipe over a surface to collect particulates from the surface"@en ;
  skos:inScheme esmat:essampletype ;
  skos:prefLabel "Dust wipe"@en ;
.
esmat:fiblamella
  rdf:type skos:Concept ;
  dcterm:source "https://osiris-rex.atlassian.net/wiki/spaces/UTDMP/pages/410288138#6.5-FIB-sections%2C-microtome-slices%2C-atom-probe-tips%2C-TEM-grids" ;
  dcterm:source "this vocabulary" ;
  rdfs:isDefinedBy esmat:essampletype ;
  rdfs:label "FIB lamella"@en ;
  skos:broader spec:analyticalpreparation ;
  skos:broader spec:solidmaterialspecimen ;
  skos:definition "very thin sheet of solid material milled from a larger sample using a focused ion beam. Used for TEM analysis."@en ;
  skos:inScheme esmat:essampletype ;
  skos:prefLabel "FIB lamella"@en ;
.
esmat:filtrate
  rdf:type skos:Concept ;
  dcterm:source "https://github.com/ess-dive-community/essdive-sample-id-metadata/blob/master/terms/objectType.md" ;
  rdfs:isDefinedBy esmat:essampletype ;
  rdfs:label "Filtrate"@en ;
  skos:broader esmat:processedfluidsample ;
  skos:definition "A sample that has gone through a filtration process to separate solids from fluids (liquids or gases), using a filter medium through which only the fluid can pass. Must be associated with a filter size."@en ;
  skos:inScheme esmat:essampletype ;
  skos:prefLabel "Filtrate"@en ;
.
esmat:glassslidesmear
  rdf:type skos:Concept ;
  dcterm:source "https://pubs.usgs.gov/of/2001/of01-041/htmldocs/methods/sslide.htm" ;
  rdfs:isDefinedBy esmat:essampletype ;
  rdfs:label "Glass slide smear"@en ;
  skos:broader spec:analyticalpreparation ;
  skos:broader spec:othersolidobject ;
  skos:definition "sample from a cell culture (or other microparticulate suspension) spread into a thin layer on a glass slide for optical investigation"@en ;
  skos:inScheme esmat:essampletype ;
  skos:prefLabel "Glass slide smear"@en ;
.
esmat:highgradesample
  rdf:type skos:Concept ;
  dcterm:source "http://earthsci.org/mineral/rockmin/sampling/sampling.html#Rock%20Sampling" ;
  rdfs:isDefinedBy esmat:essampletype ;
  rdfs:label "High Grade Sample"@en ;
  skos:broader esmat:compositesample ;
  skos:definition "in mineral exploration, selective pieces of the most highly mineralized material from a mineralize site, intentionally excluding less mineralized material. A high grade sample might be collected to indicate what the best possible values are, or to provide material for certain types of trace element analyses."@en ;
  skos:inScheme esmat:essampletype ;
  skos:prefLabel "High Grade Sample"@en ;
.
esmat:individualsolidcube
  rdf:type skos:Concept ;
  dcterm:source "SESAR vocabulary" ;
  rdfs:isDefinedBy esmat:essampletype ;
  rdfs:label "Individual solid cube"@en ;
  skos:broader spec:analyticalpreparation ;
  skos:broader spec:solidmaterialspecimen ;
  skos:definition "A sample that is a prepared cube of material, intended as a sample of that material."@en ;
  skos:inScheme esmat:essampletype ;
  skos:note "Cubes that are manufatured for decorative or utilitarian purposes should be categorized as artifacts."@en ;
  skos:prefLabel "Individual solid cube"@en ;
.
esmat:individualsolidcylinder
  rdf:type skos:Concept ;
  dcterm:source "SESAR speciment types, ODM 2" ;
  rdfs:isDefinedBy esmat:essampletype ;
  rdfs:label "Individual solid cylinder"@en ;
  skos:broader spec:solidmaterialspecimen ;
  skos:definition "A cylindrical peice of consolidated material not obtained by subsurface drilling.  Cores drilled for paleomagnetic analysis are a common example. Tree ring cores are another..."@en ;
  skos:inScheme esmat:essampletype ;
  skos:note "may be core, plug sample, drill a cylinder from a core"@en ;
  skos:prefLabel "Individual solid cylinder"@en ;
.
esmat:magneticfraction
  rdf:type skos:Concept ;
  dcterm:source "this vocabulary" ;
  rdfs:isDefinedBy esmat:essampletype ;
  rdfs:label "Magnetic fraction"@en ;
  skos:broader esmat:mineralseparate ;
  skos:broader spec:analyticalpreparation ;
  skos:definition "a collection of particles separated from a crushed rock sample based on their attraction to a magnet."@en ;
  skos:inScheme esmat:essampletype ;
  skos:prefLabel "Magnetic fraction"@en ;
.
esmat:materialcapturedinfilter
  rdf:type skos:Concept ;
  dcterm:source "https://github.com/ess-dive-community/essdive-sample-id-metadata/blob/master/terms/objectType.md" ;
  rdfs:isDefinedBy esmat:essampletype ;
  rdfs:label "Material Captured in Filter"@en ;
  skos:broader spec:genericaggregation ;
  skos:definition "A material sample captured in filter, for example from a water sample that was filtered. Must be associated with filter size field."@en ;
  skos:inScheme esmat:essampletype ;
  skos:prefLabel "Material Captured in Filter"@en ;
.
esmat:mechanicalfraction
  rdf:type skos:Concept ;
  dcterm:source "this vocabulary" ;
  rdfs:isDefinedBy esmat:essampletype ;
  rdfs:label "Mechanical fraction"@en ;
  skos:broader spec:analyticalpreparation ;
  skos:broader spec:genericaggregation ;
  skos:definition "defined by sample preparation involving mechanical processing, e.g. grain size, density, or grain shape separation."@en ;
  skos:inScheme esmat:essampletype ;
  skos:prefLabel "Mechanical fraction"@en ;
.
esmat:meteorite
  rdf:type skos:Concept ;
  dcterm:source "https://ares.jsc.nasa.gov/meteorite-falls/what-are-meteorites/" ;
  dcterm:source "https://www.iau.org/static/science/scientific_bodies/commissions/f1/meteordefinitions_approved.pdf" ;
  rdfs:label "Meteorite"@en ;
  skos:broader spec:solidmaterialspecimen ;  rdfs:isDefinedBy esmat:essampletype ;
  skos:definition "A meteorite is a solid object that originates in interplanetary space and survives passage through an atmosphere to reach the surface of a planet or moon."@en ;  skos:inScheme esmat:essampletype ;
  skos:prefLabel "Meteorite"@en ;
.
esmat:mineralseparate
  rdf:type skos:Concept ;
  dcterm:source "this vocabulary" ;
  rdfs:isDefinedBy esmat:essampletype ;
  rdfs:label "Mineral separate"@en ;
  skos:broader spec:analyticalpreparation ;
  skos:broader spec:genericaggregation ;
  skos:definition "an aggregation of particles of the same mineral extracted and concentrated from a rock."@en ;
  skos:inScheme esmat:essampletype ;
  skos:prefLabel "Mineral separate"@en ;
.
esmat:mineralspecimen
  rdf:type skos:Concept ;
  dcterm:source "this vocabulary" ;
  rdfs:isDefinedBy esmat:essampletype ;
  rdfs:label "Mineral specimen"@en ;
  skos:broader spec:solidmaterialspecimen ;
  skos:definition "a solid object consisting of one particular mineral, or several minerals intended to be representative of one or more of the mineral species."@en ;
  skos:inScheme esmat:essampletype ;
  skos:note "a sample is a 'Rock hand sample' or 'Mineral specimen' is based on whether the original collection intention is to represent a mineral species, or a rock type.  If the sample could be considered representative of a rock type or some particular mineral constitutent in the rock, classify as both."@en ;
  skos:prefLabel "Mineral specimen"@en ;
.
esmat:mountedsection
  rdf:type skos:Concept ;
  dcterm:source "this vocabulary" ;
  rdfs:isDefinedBy esmat:essampletype ;
  rdfs:label "Sectioned specimen"@en ;
  skos:broader spec:analyticalpreparation ;
  skos:broader spec:solidmaterialspecimen ;
  skos:definition "a thin slice of a solid material that has been mounted on a glass slide for study"@en ;
  skos:inScheme esmat:essampletype ;
  skos:prefLabel "Sectioned specimen"@en ;
.
esmat:naturalaggregate
  rdf:type skos:Concept ;
  dcterm:source "this vocabulary" ;
  rdfs:comment "E.g beach sand, soil, river sediment, scoop of regolith."@en ;
  rdfs:label "Natural aggregate specimen"@en ;
  skos:altLabel "Aggregate sample"@en ;  rdfs:isDefinedBy esmat:essampletype ;
  skos:broader spec:genericaggregation ;
  skos:definition "Specimen is aggregate of non-consolidated material formed by natural processes. Particles have not been intentionally modified from the sampled feature."@en ;
  skos:prefLabel "Natural aggregate specimen"@en ;  skos:inScheme esmat:essampletype ;
.
esmat:nonmagneticfraction
  rdf:type skos:Concept ;
  dcterm:source "this vocabulary" ;
  rdfs:isDefinedBy esmat:essampletype ;
  rdfs:label "Non-magnetic fraction"@en ;
  skos:broader esmat:mineralseparate ;
  skos:broader spec:analyticalpreparation ;
  skos:definition "collection of particles from a crushed rock sample based on their lack of attraction to a magnet"@en ;
  skos:inScheme esmat:essampletype ;
  skos:prefLabel "Non-magnetic fraction"@en ;
.
esmat:peel
  rdf:type skos:Concept ;
  dcterm:source "https://strata.uga.edu/cincy/fauna/bryozoanStudy/acetatePeels.html" ;
  rdfs:isDefinedBy esmat:essampletype ;
  rdfs:label "Peel"@en ;
  skos:broader spec:analyticalpreparation ;
  skos:broader spec:othersolidobject ;
  skos:definition "Acetate peels are made by polishing a planar surface on a sample, etching it with acid to give it some relief, and then chemically melting a piece of acetate onto that surface. The acetate is then pulled off for examination under a microscope. The acetate preserves a fingerprint of the internal structure of the sample surface. Used in paleontology to study complex fossils, e.g. bryozoan."@en ;
  skos:inScheme esmat:essampletype ;
  skos:prefLabel "Peel"@en ;
.
esmat:polishedmountedspecimen
  rdf:type skos:Concept ;
  dcterm:source "https://osiris-rex.atlassian.net/wiki/spaces/UTDMP/pages/410288138#6.3-Thin-section%2C-thick-section%2C-grain-mounts-(epoxy%2Fmetal-mounts)%2C-and-potted-butts" ;
  dcterm:source "this vocabulary" ;
  rdfs:label "Polished mounted specimen"@en ;  rdfs:isDefinedBy esmat:essampletype ;
  skos:altLabel "Grain mount"@en ;
  skos:broader spec:mountedspecimen ;
  skos:definition "Mounted specimen with polished surface exposing mounted material for analysis {@en}	" ;
  skos:prefLabel "Polished mounted specimen"@en ;  skos:inScheme esmat:essampletype ;
.
esmat:polishedthinsection
  rdf:type skos:Concept ;
  dcterm:source "http://www.minsocam.org/ammin/AM53/AM53_2070.pdf" ;
  rdfs:isDefinedBy esmat:essampletype ;
  rdfs:label "polished thin section"@en ;
  skos:broader esmat:thinsection ;
  skos:definition "a thin section that has its free surface polished until perfectly planar and free of pits and scratches. Used for reflected light petrography and for electron microprobe or SEM investigation."@en ;
  skos:inScheme esmat:essampletype ;
  skos:prefLabel "Polished thin section"@en ;
.
esmat:preparedpowder
  rdf:type skos:Concept ;
  dcterm:source "this vocabulary" ;
  rdfs:isDefinedBy esmat:essampletype ;
  rdfs:label "Prepared powder"@en ;
  skos:altLabel "Powder"@en ;
  skos:broader spec:analyticalpreparation ;
  skos:broader spec:genericaggregation ;
  skos:definition "distinguish from particulate in that particulate is sampled as a micron-size aggregate, whereas this material is ground to a powder for subsequent analysis; it is a powder as a function of some preparation process (e.g. chemical precipitation)"@en ;
  skos:inScheme esmat:essampletype ;
  skos:prefLabel "Prepared powder"@en ;
.
esmat:preparedrockpowder
  rdf:type skos:Concept ;
  dcterm:source "https://www.geosamples.org/vocabularies/sample-type-object" ;
  rdfs:isDefinedBy esmat:essampletype ;
  rdfs:label "Prepared rock powder"@en ;
  skos:broader esmat:preparedpowder ;
  skos:definition "a powder manufactured by pulverizing a rock."@en ;
  skos:inScheme esmat:essampletype ;
  skos:prefLabel "Prepared rock powder"@en ;
.
esmat:pressedpellet
  rdf:type skos:Concept ;
  dcterm:source "this vocabulary" ;
  rdfs:isDefinedBy esmat:essampletype ;
  rdfs:label "Pressed pellet"@en ;
  skos:broader spec:analyticalpreparation ;
  skos:broader spec:solidmaterialspecimen ;
  skos:definition "a sample prepared by grinding a parent sample to a fine powder, mixing it with a binder, and pressing the mixture into a die at a pressure of between 15 and 35 tons to produce a solid disc for subsequent analysis, typically by X-Ray fluorescence."@en ;
  skos:inScheme esmat:essampletype ;
  skos:prefLabel "Pressed pellet"@en ;
.
esmat:processedfluidsample
  rdf:type skos:Concept ;
  dcterm:source "this vocabulary" ;  rdfs:isDefinedBy esmat:essampletype ;
  rdfs:label "Processed fluid sample"@en ;  skos:inScheme esmat:essampletype ;
  skos:broader spec:fluidincontainer ;
  skos:definition "fluid sample that has been processed in some way during or after collection, e.g. by filtering, addition of preservatives."@en ;
  skos:prefLabel "Processed fluid sample"@en ;
.
esmat:residualmaterial
  rdf:type skos:Concept ;
  dcterm:source "this vocabulary" ;
  rdfs:label "Residual material"@en ;  skos:inScheme esmat:essampletype ;
  skos:altLabel "Residue"@en ;  rdfs:isDefinedBy esmat:essampletype ;
  skos:broader spec:analyticalpreparation ;
  skos:definition "Sample is material remaining after processing to extract some other components of interest from the sample."@en ;
  skos:prefLabel "Residual material"@en ;
.
esmat:rockhandsample
  rdf:type skos:Concept ;
  dcterm:source "this vocabulary" ;
  rdfs:isDefinedBy esmat:essampletype ;
  rdfs:label "Rock hand sample"@en ;
  skos:broader spec:solidmaterialspecimen ;
  skos:definition "individual peice of rock broken from an outcrop or larger peice of rock."@en ;
  skos:inScheme esmat:essampletype ;
  skos:note "use this category for rough peices of rock that have not undergone any preparation processing (crushing, sawing, etching...)"@en ;
  skos:prefLabel "Rock hand sample"@en ;
.
esmat:essampletype
  rdf:type owl:Ontology ;
  rdf:type skos:ConceptScheme ;
  rdf:type schema:CreativeWork ;
  dcterm:contributor <https://orcid.org/0000-0001-6041-5302> ;
  dcterm:created "2023-07-01"^^xsd:date ;
  dcterm:creator <https://orcid.org/0000-0001-6041-5302> ;
  dcterm:modified "2023-07-27"^^xsd:date ;
  dcterm:publisher "iSamples project" ;
  rdfs:label "Earth and Environmental Science specimen type extension"@en ;
  owl:imports dcterm: ;
  owl:imports <http://www.w3.org/2004/02/skos/core> ;
  owl:imports spec:specimentypevocabulary ;
  skos:definition "This concept scheme contains skos concepts for categorizing kinds of Earth Material sample types, extending the iSamples Material Sample Type vocabulary. Defintions from SESAR, ODM2, wikipedia, ESS-DIVE, and other sources; sources are cited with each term."@en ;
  skos:historyNote "2023-07-07 SMR add solid material sample and broader relations from classes it subsumes."@en ;
  skos:historyNote "2023-07-27 SMR modify base specimen type vocabulary, add 'Non biologic solid object' to replace 'solid material sample', change broader relations in this vocab to use that as parent class where appropriate. 'Solid material sample' is too closely linked to material type, created confusion. Intention is a specimen category for solid objects that are not biologic. Obviously there is some overlap with Research specimens."@en ;
  skos:prefLabel "Earth and Environmental Science specimen type extension"@en ;
  schema:funding <AWDID:2004562> ;
  schema:provider "TBD" ;
.
esmat:sitecompositesample
  rdf:type skos:Concept ;
  dcterm:source "http://earthsci.org/mineral/rockmin/sampling/sampling.html#Rock%20Sampling" ;
  rdfs:isDefinedBy esmat:essampletype ;
  rdfs:label "Site composite sample"@en ;
  skos:broader esmat:compositesample ;
  skos:definition "an aggregation of peices of uniform material collected over some area (generally greater than 2.5m across). These are the ideal 'representative' samples used in mineral exploration. A composite sample might be collected to determine the background values of trace elements in a particular type of rock, or to determine if ore grade mineralization is present over a large area."@en ;
  skos:inScheme esmat:essampletype ;
  skos:prefLabel "Site composite sample"@en ;
.
esmat:slab
  rdf:type skos:Concept ;
  dcterm:source "this vocabulary" ;
  rdfs:isDefinedBy esmat:essampletype ;
  rdfs:label "Slab"@en ;
  skos:broader spec:analyticalpreparation ;
  skos:broader spec:solidmaterialspecimen ;
  skos:definition "a relatively planar rock sample,cut from a large sample to produce a tabular peice of rock with the irregular outline of the original sample on the diameter where the cut was mate."@en ;
  skos:inScheme esmat:essampletype ;
  skos:prefLabel "Slab"@en ;
.
esmat:thicksection
  rdf:type skos:Concept ;
  dcterm:source "https://viva.pressbooks.pub/analyticalmethodsingeosciences/chapter/2-2-thin-section-and-thick-section-anatomy/" ;
  rdfs:isDefinedBy esmat:essampletype ;
  rdfs:label "Thick section"@en ;
  skos:broader esmat:mountedsection ;
  skos:definition "Thick sections are like thin sections, but milled to a greater thickness. Typcially polished on one or both sides and used for fluid or melt inclusion studies, Raman analyses, and infrared spectroscopy analyses, and SEM or electron microprobe. The standard thickness for a fluid inclusion thick section is 50 micrometers, but thick sections can be made at any thickness.  Thick sections can be attached to a glass slide, or can be prepared so that they can be removed from their mount as a stand-alone slice of rock."@en ;
  skos:inScheme esmat:essampletype ;
  skos:prefLabel "Thick section"@en ;
.
esmat:thinsection
  rdf:type skos:Concept ;
  dcterm:source " https://en.wikipedia.org/wiki/Thin_section" ;
  dcterm:source "http://vocabulary.odm2.org/specimentype/thinSection/ " ;
  rdfs:isDefinedBy esmat:essampletype ;
  rdfs:label "Thin section"@en ;
  skos:broader esmat:mountedsection ;
  skos:definition "thin sliver of rock cut from a sample with a diamond saw and ground optically flat, and then mounted on a glass slide and ground smooth using progressively finer abrasive grit until the sample is 30 microns thick."@en ;
  skos:inScheme esmat:essampletype ;
  skos:prefLabel "Thin section"@en ;
.
esmat:trawl
  rdf:type skos:Concept ;
  dcterm:source "this vocabulary" ;
  rdfs:isDefinedBy esmat:essampletype ;
  rdfs:label "Trawl"@en ;
  skos:broader spec:genericaggregation ;
  skos:definition "an aggregation of biogenic or non-biogenic material extracted from a water body"@en ;
  skos:inScheme esmat:essampletype ;
  skos:prefLabel "Trawl"@en ;
.
esmat:uchannelsample
  rdf:type skos:Concept ;
  dcterm:source "https://www.geosamples.org/vocabularies/sample-type-object" ;
  rdfs:isDefinedBy esmat:essampletype ;
  rdfs:label "U-channel sample"@en ;
  skos:broader spec:solidmaterialspecimen ;
  skos:definition "a rectangular prism of loosely consolidated sediment extracted from a core segment. has parent core piece or core segment"@en ;
  skos:inScheme esmat:essampletype ;
  skos:prefLabel "U-channel sample"@en ;
.
esmat:ultrathinsection
  rdf:type skos:Concept ;
  dcterm:source "http://vocabulary.odm2.org/specimentype/thinSection/  | https://en.wikipedia.org/wiki/Thin_section" ;
  rdfs:isDefinedBy esmat:essampletype ;
  rdfs:label "Ultra thin section"@en ;
  skos:broader esmat:mountedsection ;
  skos:definition "An ordinary thin section that is attached to the glass slide using a soluble cement such as Canada balsam (soluble in ethanol) to allow both sides to be worked on. The section is polished on both sides using a fine diamond paste until it has a thickness in the range of 2-12 microns. This technique has been used to study the microstructure of very fine-grained carbonate rocks, and also in the preparation of mineral and rock specimens for transmission electron microscopy."@en ;
  skos:inScheme esmat:essampletype ;
  skos:prefLabel "Ultra thin section"@en ;
.
spec:analyticalpreparation
  skos:topConceptOf esmat:essampletype ;
  skos:prefLabel "Analytical preparation"@en ;
.
spec:atomprobetip
  rdf:type skos:Concept ;
  dcterm:source "OSIRIS-Rex Sample types" ;
  dcterm:source "https://osiris-rex.atlassian.net/wiki/spaces/UTDMP/pages/410288138#6.5-FIB-sections%2C-microtome-slices%2C-atom-probe-tips%2C-TEM-grids" ;
  rdfs:label "Atom probe tip"@en ;
  skos:broader spec:solidmaterialspecimen ;  skos:inScheme esmat:essampletype ;
  skos:definition "needle-shaped sample milled out of a larger sample with a focused ion beam (FIB)."@en ;
  skos:prefLabel "Atom probe tip"@en ;  rdfs:isDefinedBy esmat:essampletype ;
.
spec:bundlebiomeaggregation
  skos:topConceptOf esmat:essampletype ;
  skos:prefLabel "Bundle biome aggregation"@en;
.
spec:chip
  rdf:type skos:Concept ;
  dcterm:source "OSIRIS-Rex Sample types" ;
  dcterm:source "https://osiris-rex.atlassian.net/wiki/spaces/UTDMP/pages/410288138/SAMIS-JSC+Curation+Interface+Control+Document+ICD#6.1-Particles-and-chips" ;
  rdfs:label "Chip"@en ;  rdfs:isDefinedBy esmat:essampletype ;
  skos:broader spec:solidmaterialspecimen ;  skos:inScheme esmat:essampletype ;
  skos:definition "Individual solid object intentionally broken off a larger solid object sample. A Chip must have a documented parent sample. {@en} " ;
  skos:prefLabel "Chip"@en ;
.
spec:eluate
  rdf:type skos:Concept ;
  dcterm:source "OSIRIS-Rex Sample types" ;
  dcterm:source "https://en.wikipedia.org/wiki/Elution" ;
  dcterm:source "https://osiris-rex.atlassian.net/wiki/spaces/UTDMP/pages/410288138#6.6-Liquids-and-Washes" ;
  rdfs:label "Eluate"@en ;  rdfs:isDefinedBy esmat:essampletype ;
  skos:broader esmat:dissolvedchemicalfraction ;
  skos:definition "The fluid product that contains the analyte of interest washed from a chromatography column"@en ;
  skos:prefLabel "Eluate"@en ;  skos:inScheme esmat:essampletype ;
.
spec:fluidincontainer
  skos:topConceptOf esmat:essampletype ;
  skos:prefLabel "Fluid in container"@en ;
.
spec:genericaggregation
  skos:topConceptOf esmat:essampletype ;
  skos:prefLabel "genericAggregation"@en
.
spec:microtomeslice
  rdf:type skos:Concept ;
  dcterm:source "OSIRIS-Rex Sample types" ;  skos:inScheme esmat:essampletype ;
  dcterm:source "https://osiris-rex.atlassian.net/wiki/spaces/UTDMP/pages/410288138#6.5-FIB-sections%2C-microtome-slices%2C-atom-probe-tips%2C-TEM-grids" ;
  rdfs:comment "Typically from TEM analysis. Slices are commonly deposited in a grid contain with multiple slices and the grid will be given a single sample name, not the individual slices within it. The provenance of the slice from paticle to mounted specimen to slice should be carefully documented"@en ;
  rdfs:label "Microtome slice "@en ;  rdfs:isDefinedBy esmat:essampletype ;
  skos:broader spec:solidmaterialspecimen ;
  skos:definition "A very thin slice cut from a mounted specimen using a mocrotome or ultramicrotome."@en ;
  skos:prefLabel "Microtome slice"@en ;
.
spec:mountedspecimen
  rdf:type skos:Concept ;
  dcterm:source "OSIRIS-Rex Sample types" ;
  dcterm:source "https://osiris-rex.atlassian.net/wiki/spaces/UTDMP/pages/410288138#6.3-Thin-section%2C-thick-section%2C-grain-mounts-(epoxy%2Fmetal-mounts)%2C-and-potted-butts" ;
  rdfs:label "Mounted specimen"@en ;  skos:inScheme esmat:essampletype ;
  skos:altLabel "Potted butt"@en ;  rdfs:isDefinedBy esmat:essampletype ;
  skos:broader spec:solidmaterialspecimen ;
  skos:definition "one or more solid objects embedded in a stabilizing matrix, typically epoxy, metal, or paraffin to allow slicing through the mounted object(s)."@en ;
  skos:prefLabel "Mounted specimen"@en ;
.
spec:othersolidobject
  skos:topConceptOf esmat:essampletype ;
  skos:prefLabel "Other solid Object"@en ;
.
spec:particle
  rdf:type skos:Concept ;
  dcterm:source "OSIRIS-Rex Sample types" ;  skos:inScheme esmat:essampletype ;
  dcterm:source "https://osiris-rex.atlassian.net/wiki/spaces/UTDMP/pages/410288138/SAMIS-JSC+Curation+Interface+Control+Document+ICD#6.1-Particles-and-chips" ;
  rdfs:comment "Can also used for small peices broken from a 'Rock hand sample'.   OSIRIS-Rex definition specifies 'competent individual geologic sample of any size'. 'Competent' interpreted to be equivalent to 'solid', or 'consolidated'.  The definition here is broader in that it includes materials of any origin, but narrower in that it is restricted to small objects."@en ;
  rdfs:label "Particle"@en ;  rdfs:isDefinedBy esmat:essampletype ;
  skos:broader spec:solidmaterialspecimen ;
  skos:definition "A small individual solid object that is not one of the other sample types."@en ;
  skos:prefLabel "Particle"@en ;
.
spec:temgrid
  rdf:type skos:Concept ;
  dcterm:source "OSIRIS-Rex Sample types" ;  skos:inScheme esmat:essampletype ;
  dcterm:source "https://osiris-rex.atlassian.net/wiki/spaces/UTDMP/pages/410288138#6.5-FIB-sections%2C-microtome-slices%2C-atom-probe-tips%2C-TEM-grids" ;
  rdfs:label "TEM grid "@en ;  rdfs:isDefinedBy esmat:essampletype ;
  skos:broader spec:genericaggregation ;
  skos:definition "FIB sections and microtome slices set onto a small grid for handling, transport, and analysis using a transmission electron microscope (TEM). The grid itself can be given a single sample identifier (similar to how there are multiple grains in a grain mount). The linkage from the individual samples in the grid to their parent sample(s) should be documented"@en ;
  skos:prefLabel "Resonance ionization mass spectrometry" ;
.
