# baseURI: https://w3id.org/isample/1.0/sampledfeaturerole/sfrolevocabulary
# imports: http://purl.org/dc/terms/
# imports: http://www.w3.org/2004/02/skos/core

@prefix dcterm: <http://purl.org/dc/terms/> .
@prefix essfrole: <https://w3id.org/isample/1.0/sampledfeaturerole/> .
@prefix owl: <http://www.w3.org/2002/07/owl#> .
@prefix rdf: <http://www.w3.org/1999/02/22-rdf-syntax-ns#> .
@prefix rdfs: <http://www.w3.org/2000/01/rdf-schema#> .
@prefix schema: <https://schema.org/> .
@prefix skos: <http://www.w3.org/2004/02/skos/core#> .
@prefix xsd: <http://www.w3.org/2001/XMLSchema#> .

<essfrole:2004562>
  rdf:type schema:Grant ;
  schema:funder <https://ror.org/04nh1dc89> ;
  schema:name "Collaborative Research: Frameworks: Internet of Samples: Toward an Interdisciplinary Cyberinfrastructure for Material Samples" ;
  schema:url "https://nsf.gov/awardsearch/showAward?AWD_ID=2004562" ;
.
essfrole:cement
  rdf:type skos:Concept ;
  dcterm:source "This vocabulary" ;
  rdfs:isDefinedBy essfrole:sfrolevocabulary ;
  rdfs:label "cement"@en ;
  skos:broader essfrole:individualconstituent ;
  skos:definition "sampled feature is material that binds constituent particles together in a sedimentary rock."@en ;
  skos:inScheme essfrole:sfrolevocabulary ;
  skos:prefLabel "cement"@en ;
.
essfrole:clast
  rdf:type skos:Concept ;
  dcterm:source "This vocabulary" ;
  rdfs:isDefinedBy essfrole:sfrolevocabulary ;
  rdfs:label "clast"@en ;
  skos:broader essfrole:inclusion ;
  skos:definition "A clast is a fragment of rock or mineral derived from some pre-existing rock or generated by intrabasinal processes that is a part of a sediment"@en ;
  skos:inScheme essfrole:sfrolevocabulary ;
  skos:prefLabel "clast"@en ;
.
essfrole:cognateinclusion
  rdf:type skos:Concept ;
  dcterm:source "This vocabulary" ;
  rdfs:isDefinedBy essfrole:sfrolevocabulary ;
  rdfs:label "cognate inclusion"@en ;
  skos:altLabel "autolith"@en ;
  skos:broader essfrole:inclusion ;
  skos:definition "An inclusion in an igneous rock that is interpreted to be genetically related to the enclosing rock."@en ;
  skos:inScheme essfrole:sfrolevocabulary ;
  skos:prefLabel "cognate inclusion"@en ;
.
essfrole:fluidinclusion
  rdf:type skos:Concept ;
  dcterm:source "This vocabulary" ;
  rdfs:isDefinedBy essfrole:sfrolevocabulary ;
  rdfs:label "fluid inclusion"@en ;
  skos:broader essfrole:inclusion ;
  skos:definition "an inclusion that is an opening in a mineral grain containing fluid (liquid or gas)."@en ;
  skos:inScheme essfrole:sfrolevocabulary ;
  skos:prefLabel "fluid inclusion"@en ;
.
essfrole:groundmass
  rdf:type skos:Concept ;
  dcterm:source "This vocabulary" ;
  rdfs:isDefinedBy essfrole:sfrolevocabulary ;
  rdfs:label "groundmass"@en ;
  skos:broader essfrole:individualconstituent ;
  skos:definition "sampled feature is fine-grained to aphanitic material that is interstitial to larger crystals or particles in a sample."@en ;
  skos:inScheme essfrole:sfrolevocabulary ;
  skos:prefLabel "groundmass"@en ;
.
essfrole:inclusion
  rdf:type skos:Concept ;
  dcterm:source "this vocabulary" ;
  rdfs:label "inclusion"@en ;
  skos:broader essfrole:sampledfeaturepart ;
  skos:definition "sampled feature is an object contained within a larger body of material."@en ;
  skos:example "fluid inclusion, xenolith, clast in a sedimentary material."@en ;
  skos:prefLabel "inclusion"@en ;
.
essfrole:individualconstituent
  rdf:type skos:Concept ;
  dcterm:source "This vocabulary" ;
  rdfs:isDefinedBy essfrole:sfrolevocabulary ;
  rdfs:label "individual constituent"@en ;
  skos:broader essfrole:sampledfeaturepart ;
  skos:definition "sampled feature is a single particle or collection of particles that share some characteristic, within or extracted from a larger sample."@en ;
  skos:example "mineral separate, point analysis of particular particles"@en ;
  skos:inScheme essfrole:sfrolevocabulary ;
  skos:prefLabel "individual constituent"@en ;
.
essfrole:meltinclusion
  rdf:type skos:Concept ;
  dcterm:source "This vocabulary" ;
  rdfs:isDefinedBy essfrole:sfrolevocabulary ;
  rdfs:label "melt inclusion"@en ;
  skos:broader essfrole:inclusion ;
  skos:definition "An inclusion in a mineral grain in an igneous rock that is interpreted to consist of trapped magma from which the igneous rock was formed."@en ;
  skos:inScheme essfrole:sfrolevocabulary ;
  skos:prefLabel "melt inclusion"@en ;
.
essfrole:mineralinclusion
  rdf:type skos:Concept ;
  dcterm:source "This vocabulary" ;
  rdfs:isDefinedBy essfrole:sfrolevocabulary ;
  rdfs:label "mineral inclusion"@en ;
  skos:broader essfrole:inclusion ;
  skos:definition "An inclusion of a mineral phase contained inside a grain of another mineral."@en ;
  skos:inScheme essfrole:sfrolevocabulary ;
  skos:prefLabel "mineral inclusion"@en ;
.
essfrole:sfrolevocabulary
  rdf:type owl:Ontology ;
  rdf:type skos:ConceptScheme ;
  rdf:type schema:CreativeWork ;
  dcterm:contributor <https://orcid.org/0000-0001-6041-5302> ;
  dcterm:created "2023-11-17"^^xsd:date ;
  dcterm:creator <https://orcid.org/0000-0001-6041-5302> ;
  dcterm:modified "2023-11-17"^^xsd:date ;
  dcterm:publisher "iSamples project" ;
  rdfs:label "Earth and Environmental Science sampled feature role extension"@en ;
  owl:imports dcterm: ;
  owl:imports <http://www.w3.org/2004/02/skos/core> ;
  skos:definition "Terms to categorize the relation of a sampled feature to its context. In the Earth Science realm this is typically relation of sampled feature to a containing rock body or rock body part."@en ;
  skos:hasTopConcept essfrole:sampledfeaturepart ;
  skos:historyNote "2023-11-17 SMR generate to account for sample classifications in SESAR"@en ;
  skos:prefLabel "Earth and Environmental Science sampled feature role extension"@en ;
  schema:funding <essfrole:2004562> ;
  schema:provider "TBD" ;
.
essfrole:phenocryst
  rdf:type skos:Concept ;
  dcterm:source "This vocabulary" ;
  rdfs:isDefinedBy essfrole:sfrolevocabulary ;
  rdfs:label "phenocryst"@en ;
  skos:broader essfrole:individualconstituent ;
  skos:definition "Sampled feature is a crystal that is significantly larger than surrounding crystals in an igneous rock."@en ;
  skos:inScheme essfrole:sfrolevocabulary ;
  skos:prefLabel "phenocryst"@en ;
.
essfrole:porphyroblast
  rdf:type skos:Concept ;
  dcterm:source "This vocabulary" ;
  rdfs:isDefinedBy essfrole:sfrolevocabulary ;
  rdfs:label "porphyroblast"@en ;
  skos:broader essfrole:individualconstituent ;
  skos:definition "Sampled feature is a crystal that is significantly larger than surrounding crystals in a metamorphic rock."@en ;
  skos:inScheme essfrole:sfrolevocabulary ;
  skos:prefLabel "porphyroblast"@en ;
.
essfrole:rockbody
  rdf:type skos:Concept ;
  dcterm:source "This vocabulary" ;
  rdfs:isDefinedBy essfrole:sfrolevocabulary ;
  rdfs:label "rock body"@en ;
  skos:broader essfrole:sampledfeaturepart ;
  skos:definition "sampled feature is representative of a rock body, i.e. it represents the whole of the sampled body."@en ;
  skos:inScheme essfrole:sfrolevocabulary ;
  skos:prefLabel "rock body"@en ;
.
essfrole:sampledfeaturepart
  rdf:type skos:Concept ;
  dcterm:source "this vocabulary" ;
  rdfs:label "Sampled feature part"@en ;
  skos:definition "A sampled feature that is part of a larger sampled feature; Could be improper part (e.g. the whole larger feature)"@en ;
  skos:prefLabel "Sampled feature part" ;
  skos:topConceptOf essfrole:sfrolevocabulary ;
.
essfrole:xenolith
  rdf:type skos:Concept ;
  dcterm:source "This vocabulary" ;
  rdfs:isDefinedBy essfrole:sfrolevocabulary ;
  rdfs:label "xenolith"@en ;
  skos:broader essfrole:inclusion ;
  skos:definition "An inclusion that is a fragment of pre-existing material that is contained in an igneous rock and unrelated to the magma that formed the rock."@en ;
  skos:inScheme essfrole:sfrolevocabulary ;
  skos:prefLabel "xenolith"@en ;
.
